module Auto.Induction where

open import Data.Vec
open import Data.Fin hiding (_+_)
open import Data.Nat renaming (_≟_ to _≟-Nat_)
open import Data.Product
open import Data.List
open import Relation.Binary.PropositionalEquality
open import Relation.Binary
open import Relation.Nullary
open import Function

open import Auto.Expr
open import Auto.ProofDatatypes
open import Auto.Normalization
open import Auto.Instantiation

private
  -- Induction ------------------------------------------------------------------
  induction-inst : {n : ℕ} (lhs rhs : Expr (suc n))
                 → Equality (inst-zero lhs) (inst-zero rhs)
                 → (∀ Γ → ⟦ lhs ⟧ Γ ≡ ⟦ rhs ⟧ Γ
                        → ⟦ inst-suc lhs ⟧ Γ ≡ ⟦ inst-suc rhs ⟧ Γ)
                 → Equality lhs rhs
  induction-inst lhs rhs p0 ps (zero ∷ Γ)  = sym (inst-zero-correct lhs Γ) ⟨ trans ⟩
                                             p0 Γ                          ⟨ trans ⟩
                                             inst-zero-correct rhs Γ
  induction-inst lhs rhs p0 ps (suc k ∷ Γ) = sym (inst-suc-correct k lhs Γ)                    ⟨ trans ⟩
                                             ps (k ∷ Γ) (induction-inst lhs rhs p0 ps (k ∷ Γ)) ⟨ trans ⟩
                                             inst-suc-correct k rhs Γ

  -- If the expressions are equal, then so is evaluating them under the same environment
  cong-⟦─⟧ : {n : ℕ} {e₁ e₂ : Expr n} (Γ : Env n) → e₁ ≡ e₂ → ⟦ e₁ ⟧ Γ ≡ ⟦ e₂ ⟧ Γ
  cong-⟦─⟧ Γ = cong (λ e → ⟦ e ⟧ Γ)

  -- Instantiates the first lemma that matches in the given direction
  inst-lemma : {n : ℕ} → LR → List Lemma → (e : Expr n) → Try (∃ (Equality e))
  inst-lemma     lr []                        e = fail (lemma-failed e)
  inst-lemma {n} lr (lemma m lhs rhs eq ∷ ls) e with n ≟-Nat m
  ... | no ¬p = inst-lemma lr ls e
  inst-lemma lr    (lemma m lhs rhs eq ∷ ls) e | yes refl with e ≟ lhs | e ≟ rhs
  inst-lemma left  (lemma m lhs rhs eq ∷ ls) e | yes refl | yes p | _ = success (lemmaStep rhs) (rhs , λ Γ → cong-⟦─⟧ Γ p ⟨ trans ⟩ eq Γ)
  inst-lemma right (lemma m lhs rhs eq ∷ ls) e | yes refl | _ | yes p = success (lemmaStep lhs) (lhs , λ Γ → cong-⟦─⟧ Γ p ⟨ trans ⟩ sym (eq Γ))
  ... | _ | _ = inst-lemma lr ls e

  -- Instantiate the induction hypothesis. Match the goal with the given. -------
  induction-step : {n : ℕ}
          → ℕ → List Lemma
          → (hl hr sl sr : Expr (suc n))
          → Try (∀ Γ → ⟦ hl ⟧ Γ ≡ ⟦ hr ⟧ Γ → ⟦ sl ⟧ Γ ≡ ⟦ sr ⟧ Γ)
  induction-step uses lemmas hl hr sl sr with sl ≟ sr | sl ≟ hl | hr ≟ sr
  -- The step sides match
  ... | yes s-eq | _        | _        = success stepSideMatch λ Γ _  → cong-⟦─⟧ Γ s-eq
  -- The step sides match the induction hypothesis
  ... | _        | yes l-eq | yes r-eq = success stepMatchIH λ Γ ih → cong-⟦─⟧ Γ l-eq ⟨ trans ⟩ ih ⟨ trans ⟩ cong-⟦─⟧ Γ r-eq

  {-
  -- The left step side match the induction hypothesis  (this could be nice to use)
  ... | _        | yes l-eq | no ¬p    = ...
  -- The right step side match the induction hypothesis (this could be nice to use)
  ... | _        | no ¬p    | yes r-eq = ...
  -}

  -- The step sides both start with suc
  induction-step uses lemmas hl hr (suc sl)  (suc sr)  | _ | _ | _ with induction-step uses lemmas hl hr sl sr
  ... | success t p = success (stepSuc t) λ Γ ih → cong suc (p Γ ih)
  ... | fail e    = fail e
  -- The step sides both start with ⊕
  induction-step uses lemmas hl hr (l₁ ⊕ l₂) (r₁ ⊕ r₂) | _ | _ | _ with induction-step uses lemmas hl hr l₁ r₁ | induction-step uses lemmas hl hr l₂ r₂
  ... | success t₁ p₁ | success t₂ p₂ = success (t₁ stepPlus t₂) λ Γ ih → p₁ Γ ih ⟨ cong₂ _+_ ⟩ p₂ Γ ih
  ... | _             | _             = fail (step-failed hl hr (l₁ ⊕ l₂) (r₁ ⊕ r₂))
  -- No lemmas uses left
  induction-step zero         lemmas hl hr sl sr | _ | _ | _ = fail (step-failed hl hr sl sr)
  -- Instantiate a lemma
  induction-step (suc uses-1) lemmas hl hr sl sr | _ | _ | _ with inst-lemma left lemmas sl | inst-lemma right lemmas sr
  ... | success t (sl′ , sl≡sl′) | _ = (λ ih' Γ ih → sl≡sl′ Γ ⟨ trans ⟩ ih' Γ ih)
                                  <$>⟨ apply t ⟩ induction-step uses-1 lemmas hl hr sl′ sr
  ... | _ | success t (sr′ , sr≡sr′) = (λ ih' Γ ih → ih' Γ ih ⟨ trans ⟩ sym (sr≡sr′ Γ))
                                  <$>⟨ apply t ⟩ induction-step uses-1 lemmas hl hr sl sr′
  ... | _ | _ = fail (no-lemmas-left (step-failed hl hr sl sr))

  -- Simplifylification. ------------------------------------------------------------
  -- Used for the base case and for proving equality with no variables
  simplify : {n : ℕ}
       → ℕ → List Lemma
       → (lhs rhs : Expr n)
       -- ^ normalized lhs and rhs
       → Try (Equality lhs rhs)
  simplify uses lemmas lhs rhs with lhs ≟ rhs
  -- lhs ≡ rhs by reflexivity
  ... | yes p = success refl (λ Γ → cong-⟦─⟧ Γ p)
  -- No lemma uses left
  simplify zero         lemmas lhs rhs | no ¬p = fail (no-lemmas-left (simplify-failed lhs rhs))
  -- Try to use a lemma
  simplify (suc uses-1) lemmas lhs rhs | no ¬p with inst-lemma left lemmas lhs | inst-lemma right lemmas rhs
  ... | success t (lhs′ , lhs≡lhs′) | _ = (λ x Γ → lhs≡lhs′ Γ ⟨ trans ⟩ x Γ)
                                        <$>⟨ apply t ⟩ simplify uses-1 lemmas lhs′ rhs
  ... | _ | success t (rhs′ , rhs≡rhs′) = (λ x Γ → x Γ ⟨ trans ⟩ sym (rhs≡rhs′ Γ))
                                        <$>⟨ apply t ⟩ simplify uses-1 lemmas lhs rhs′
  ... | _ | _ = fail (simplify-failed lhs rhs)

  -- Induction on the first variable --------------------------------------------
  induction : {n : ℕ}
            → ℕ → List Lemma
            → (lhs rhs : Expr (suc n)) → Try (Equality lhs rhs)
  induction uses lemmas lhs rhs with simplify uses lemmas (normalize (inst-zero lhs))
                                                      (normalize (inst-zero rhs))
  -- Base case failed
  ... | fail e = fail (base-failed e)
  -- Base case suceeded
  ... | success tb base with induction-step uses lemmas (normalize lhs) (normalize rhs)
                                                 (normalize (inst-suc lhs))
                                                 (normalize (inst-suc rhs))
  -- Induction step suceeded
  ... | success th ih-norm = success base⟨ tb ⟩step⟨ th ⟩
                                (induction-inst lhs rhs
                                   (λ Γ → normalize-correct (inst-zero lhs) Γ         ⟨ trans ⟩
                                          base Γ                                      ⟨ trans ⟩
                                          sym (normalize-correct (inst-zero rhs) Γ))
                                   (λ Γ ih → normalize-correct (inst-suc lhs) Γ       ⟨ trans ⟩
                                             ih-norm Γ (sym (normalize-correct lhs Γ) ⟨ trans ⟩
                                                       ih                             ⟨ trans ⟩
                                                       normalize-correct rhs Γ )      ⟨ trans ⟩
                                             sym (normalize-correct (inst-suc rhs) Γ)))
  -- Induction step failed
  ... | fail e = fail e

-- Prove a property with lemmas -----------------------------------------------
prove-with-lemmas : (n : ℕ) (lhs rhs : Expr n)
                  → ℕ → List Lemma
                  → Try (Equality lhs rhs)
prove-with-lemmas (suc n) lhs rhs u lemmas = induction u lemmas lhs rhs
prove-with-lemmas zero    lhs rhs u lemmas = (λ x Γ → normalize-correct lhs Γ ⟨ trans ⟩
                                                      x Γ                     ⟨ trans ⟩
                                                      sym (normalize-correct rhs Γ))
                                            <$>⟨ id ⟩ simplify u lemmas (normalize lhs) (normalize rhs)


-- Prove a property without lemmas --------------------------------------------
prove : (n : ℕ) (lhs rhs : Expr n) → Try (Equality lhs rhs)
prove n lhs rhs = prove-with-lemmas n lhs rhs 0 []

open import Auto.ReplaceZero

prove-with-induction-on-and-lemmas : (n : ℕ) (v : Fin n) (lhs rhs : Expr n)
                                   → ℕ → List Lemma
                                   → Try (Equality lhs rhs)
prove-with-induction-on-and-lemmas zero    () lhs rhs u lemmas
prove-with-induction-on-and-lemmas (suc n) v  lhs rhs u lemmas =
   reshuffle-correct lhs rhs v <$>⟨ reshuffle ⟩
   prove-with-lemmas (suc n) (place v first lhs) (place v first rhs) u lemmas

prove-with-induction-on : (n : ℕ) (v : Fin n) (lhs rhs : Expr n)
                        → Try (Equality lhs rhs)
prove-with-induction-on n v lhs rhs = prove-with-induction-on-and-lemmas n v lhs rhs 0 []
